\documentclass{article}
\usepackage[margin=0.8in]{geometry}
\usepackage[mathletters]{ucs}
\usepackage[T1]{fontenc}
\usepackage[utf8x]{inputenc}
\usepackage{mathpartir}
\usepackage{mathtools}
\usepackage{amsthm}
\usepackage{amsmath}
\usepackage{amssymb}
\usepackage{csquotes}
\usepackage{trimclip}
\usepackage{tikz-cd}
\usepackage{authblk}
\newtheorem{theorem}{Theorem}

\newcommand{\Un}{\text{U}}
\newcommand{\Ln}{\text{L}}
\newcommand{\ty}[1]{:_{#1}}
\newcommand{\tL}{:_{\text{L}}}
\newcommand{\tU}{:_{\text{U}}}
\newcommand{\PiR}[3]{\Pi_{#1}({#2}).{#3}}
\newcommand{\PiI}[3]{\Pi_{#1}\{{#2}\}.{#3}}
\newcommand{\lamR}[3]{\lambda_{#1}({#2}).{#3}}
\newcommand{\lamI}[3]{\lambda_{#1}\{{#2}\}.{#3}}
\newcommand{\SigR}[3]{\Sigma_{#1}({#2}).{#3}}
\newcommand{\SigI}[3]{\Sigma_{#1}\{{#2}\}.{#3}}
\newcommand{\pairR}[3]{\langle{{#1},{#2}}\rangle_{#3}}
\newcommand{\pairI}[3]{\{{#1},{#2}\}_{#3}}
\newcommand{\SigElim}[3]{\text{R}_{#1}^{\Sigma}({#2},{#3})}
\newcommand{\with}[3]{{#1}\;\&_{#3}{#2}}
\newcommand{\apair}[3]{({#1}, {#2})_{#3}}
\newcommand{\projL}[1]{\pi_{1}\,{#1}}
\newcommand{\projR}[1]{\pi_{2}\,{#1}}
\newcommand{\iden}[3]{{#2}\equiv_{#1}{#3}}
\newcommand{\refl}[1]{\text{refl}\;{#1}}
\newcommand{\idenElim}[3]{\text{R}_{#1}^{\equiv}({#2},{#3})}
\newcommand{\dotcup}{\ensuremath{\mathbin{\mathaccent\cdot\cup}}}
\newcommand{\fresh}[1]{\textit{fresh}({#1})}
\newcommand{\val}{\text{ value}}

\makeatletter
\newcommand*{\Leadsto}{\leadsto\joinrel\mathrel{\mathpalette\@Leadsto\relax}}
\newcommand*{\@Leadsto}[2]{%
   \clipbox{{.68\width} 0pt 0pt {-.2\height}}{$\m@th#1\leadsto$}%
}

\title{A Two Level Linear Dependent Type Theory}
\author[1]{Qiancheng Fu}
\author[1]{Hongwei Xi}
\affil[1]{Boston University}

\begin{document}

\maketitle

\section{Syntax}
\begin{center}
  \begin{tabular}{r l c l}
    variables & $x, y, z, p$    &     &               \\
    sorts     & $s, r, t$       & ::= & $\Un$ | $\Ln$ \\
    terms     & $m,n,A,B,C,H,P$ & ::= & $x$ | $s$ \\
              &                 & \;| & $\PiR{t}{x : A}{B}$ | $\PiI{t}{x : A}{B}$
                                        | $\SigR{t}{x : A}{B}$ | $\SigI{t}{x : A}{B}$
                                        | $\with{A}{B}{t}$ \\
              &                 & \;| & $\lamR{t}{x : A}{m}$ | $\lamI{t}{x : A}{m}$
                                        | $\pairR{m}{n}{t}$ | $\pairI{m}{n}{t}$ | $\apair{m}{n}{t}$  \\
              &                 & \;| & $m\ n$ | $\SigElim{[z]A}{m}{[x,y]n}$ | $\projL{m}$ | $\projR{m}$ \\
              &                 & \;| & $\iden{A}{m}{n}$ | $\refl{m}$ | $\idenElim{[x,y,p]A}{[z]H}{P}$
                                        | $\square$ \\
    values    & $u, v$          & ::= & $x$ | $\lamR{t}{x : A}{m}$ | $\lamI{t}{x : A}{m}$
                                        | $\pairR{u}{v}{t}$ | $\pairI{v}{m}{t}$ | $\apair{m}{n}{t}$
  \end{tabular}
\end{center}

\newpage

\section{Static Fragment}
\subsection*{Sort Order}
\begin{mathpar}
  \inferrule
  { }
  { \Un \sqsubseteq s }

  \inferrule
  { }
  { \Ln \sqsubseteq \Ln }
\end{mathpar}

\subsection*{Static Context}
\begin{mathpar}
  \inferrule
  {  }
  { \epsilon \vdash }

  \inferrule
  { \Gamma \vdash \\
    \Gamma \vdash A : s \\
    x \in \fresh{\Gamma} }
  { \Gamma, x : A \vdash }
\end{mathpar}

\subsection*{Static Typing}
\begin{mathpar}
  \inferrule
  { \Gamma \vdash }
  { \Gamma \vdash s : \Un }

  \inferrule
  { \Gamma, x : A \vdash }
  { \Gamma, x : A \vdash x : A }

  \inferrule
  { \Gamma \vdash A : s \\
    \Gamma, x : A \vdash B : r }
  { \Gamma \vdash \PiR{t}{x : A}{B} : t }

  \inferrule
  { \Gamma \vdash A : s \\
    \Gamma, x : A \vdash B : r }
  { \Gamma \vdash \PiI{t}{x : A}{B} : t }

  \inferrule
  { \Gamma, x : A \vdash m : B }
  { \Gamma \vdash \lamR{t}{x : A}{m} : \PiR{t}{x : A}{B} }

  \inferrule
  { \Gamma, x : A \vdash m : B }
  { \Gamma \vdash \lamI{t}{x : A}{m} : \PiI{t}{x : A}{B} }

  \inferrule
  { \Gamma \vdash m : \PiR{t}{x : A}{B} \\
    \Gamma \vdash n : A }
  { \Gamma \vdash m\ n : B[n/x] }

  \inferrule
  { \Gamma \vdash m : \PiI{t}{x : A}{B} \\
    \Gamma \vdash n : A }
  { \Gamma \vdash m\ n : B[n/x] }

  \inferrule
  { s \sqsubseteq t \\ r \sqsubseteq t \\
    \Gamma \vdash A : s \\
    \Gamma, x : A \vdash B : r }
  { \Gamma \vdash \SigR{t}{x : A}{B} : t }

  \inferrule
  { s \sqsubseteq t \\
    \Gamma \vdash A : s \\
    \Gamma, x : A \vdash B : r }
  { \Gamma \vdash \SigI{t}{x : A}{B} : t }

  \inferrule
  { \Gamma \vdash \SigR{t}{x : A}{B} \\
    \Gamma \vdash m : A \\
    \Gamma \vdash n : B[m/x] }
  { \Gamma \vdash \pairR{m}{n}{t} : \SigR{t}{x : A}{B} }

  \inferrule
  { \Gamma \vdash \SigI{t}{x : A}{B} \\
    \Gamma \vdash m : A \\
    \Gamma \vdash n : B[m/x] }
  { \Gamma \vdash \pairI{m}{n}{t} : \SigI{t}{x : A}{B} }

  \inferrule
  { \Gamma, z : \SigR{t}{x : A}{B} \vdash C : s \\
    \Gamma \vdash m : \SigR{t}{x : A}{B} \\
    \Gamma, x : A, y : B \vdash n : C[\pairR{x}{y}{t}/z] }
  { \Gamma \vdash \SigElim{[z]C}{m}{[x,y]n} : C[m/z] }

  \inferrule
  { \Gamma, z : \SigI{t}{x : A}{B} \vdash C : s \\
    \Gamma \vdash m : \SigI{t}{x : A}{B} \\
    \Gamma, x : A, y : B \vdash n : C[\pairI{x}{y}{t}/z] }
  { \Gamma \vdash \SigElim{[z]C}{m}{[x,y]n} : C[m/z] }
  \\

  \inferrule
  { \Gamma \vdash A : s \\
    \Gamma \vdash B : r }
  { \Gamma \vdash \with{A}{B}{t} : t }

  \inferrule
  { \Gamma \vdash m : A \\
    \Gamma \vdash n : B }
  { \Gamma \vdash \apair{m}{n}{t} : \with{A}{B}{t} }

  \inferrule
  { \Gamma \vdash m : \with{A}{B}{t} }
  { \Gamma \vdash \projL{m} : A }

  \inferrule
  { \Gamma \vdash m : \with{A}{B}{t} }
  { \Gamma \vdash \projR{m} : B }

  \inferrule
  { \Gamma \vdash A : s \\
    \Gamma \vdash m : A \\
    \Gamma \vdash n : A }
  { \Gamma \vdash \iden{A}{m}{n} : \Un }

  \inferrule
  { \Gamma \vdash m : A }
  { \Gamma \vdash \refl{m} : \iden{A}{m}{m} }

  \inferrule
  { \Gamma, x : A, y : A, p : \iden{A}{x}{y} \vdash B : s \\
    \Gamma, z : A \vdash H : B[z/x,z/y,\refl{z}/p] \\
    \Gamma \vdash P : \iden{A}{m}{n} }
  { \Gamma \vdash \idenElim{[x,y,p]B}{[z]H}{P} : B[m/x,n/y,P/p] }

  \inferrule
  { \Gamma \vdash B : s \\
    \Gamma \vdash m : A \\
    A \simeq B }
  { \Gamma \vdash m : B }
\end{mathpar}

\newpage

\section{Dynamic Fragment}
\subsection*{Dynamic Context}
\begin{mathpar}
  \inferrule
  { }
  { \epsilon ; \epsilon \vdash }

  \inferrule
  { \Gamma ; \Delta \vdash \\
    \Gamma \vdash A : s \\
    x \in \fresh{\Gamma} }
  { \Gamma, x : A ; \Delta, x \ty{s} A \vdash }

  \inferrule
  { \Gamma ; \Delta \vdash \\
    \Gamma \vdash A : s \\
    x \in \fresh{\Gamma} }
  { \Gamma, x : A ; \Delta \vdash }
\end{mathpar}

\subsection*{Context Merge}
\begin{mathpar}
  \inferrule
  { }
  { \epsilon \dotcup \epsilon = \epsilon }

  \inferrule
  { \Delta_1 \dotcup \Delta_2 = \Delta \\
    x \in \fresh{\Delta} }
  { (\Delta_1, x \tU A) \dotcup (\Delta_2, x \tU A) = (\Delta, x \tU A) }
  \\

  \inferrule
  { \Delta_1 \dotcup \Delta_2 = \Delta \\
    x \in \fresh{\Delta} }
  { (\Delta_1, x \tL A) \dotcup \Delta_2 = (\Delta, x \tL A) }

  \inferrule
  { \Delta_1 \dotcup \Delta_2 = \Delta \\
    x \in \fresh{\Delta} }
  { \Delta_1 \dotcup (\Delta_2, x \tL A) = (\Delta, x \tL A) }
\end{mathpar}

\subsection*{Context Constraint}
\begin{mathpar}
  \inferrule
  { }
  { \epsilon \triangleright s }

  \inferrule
  { \Delta \triangleright \Un }
  { \Delta, x \tU A \triangleright \Un }

  \inferrule
  { \Delta \triangleright \Ln }
  { \Delta, x \ty{s} A \triangleright \Ln }
\end{mathpar}

\subsection*{Dynamic Typing}
\begin{mathpar}
  \inferrule
  { \Gamma, x : A ; \Delta, x \ty{s} A \vdash \\
    \Delta \triangleright \Un }
  { \Gamma, x : A ; \Delta, x \ty{s} A \vdash x : A }

  \inferrule
  { \Gamma, x : A; \Delta, x \ty{s} A \vdash m : B \\
    \Delta \triangleright t }
  { \Gamma ; \Delta \vdash \lamR{t}{x : A}{m} : \PiR{t}{x : A}{B} }

  \inferrule
  { \Gamma, x : A; \Delta \vdash m : B \\
    \Delta \triangleright t }
  { \Gamma ; \Delta \vdash \lamI{t}{x : A}{m} : \PiI{t}{x : A}{B} }

  \inferrule
  { \Gamma ; \Delta_1 \vdash m : \PiR{t}{x : A}{B} \\
    \Gamma ; \Delta_2 \vdash n : A }
  { \Gamma ; \Delta_1 \dotcup \Delta_2 \vdash m\ n : B[n/x] }

  \inferrule
  { \Gamma ; \Delta \vdash m : \PiI{t}{x : A}{B} \\
    \Gamma \vdash n : A }
  { \Gamma ; \Delta \vdash m\ n : B[n/x] }

  \inferrule
  { \Gamma \vdash \SigR{t}{x : A}{B} : t \\
    \Gamma ; \Delta_1 \vdash m : A \\
    \Gamma ; \Delta_2 \vdash n : B[m/x] }
  { \Gamma ; \Delta_1 \dotcup \Delta_2 \vdash \pairR{m}{n}{t} : \SigR{t}{x : A}{B} }

  \inferrule
  { \Gamma \vdash \SigI{t}{x : A}{B} : t \\
    \Gamma ; \Delta \vdash m : A \\
    \Gamma \vdash n : B[m/x] }
  { \Gamma ; \Delta \vdash \pairI{m}{n}{t} : \SigI{t}{x : A}{B} }

  \inferrule
  { \Gamma, z : \SigR{t}{x : A}{B} \vdash C : s \\
    \Gamma ; \Delta_1 \vdash m : \SigR{t}{x : A}{B} \\
    \Gamma, x : A, y : B; \Delta_2, x \ty{r1} A, y \ty{r2} B \vdash n : C[\pairR{x}{y}{t}/z] }
  { \Gamma ; \Delta_1 \dotcup \Delta_2 \vdash \SigElim{[z]C}{m}{[x,y]n} : C[m/z] }

  \inferrule
  { \Gamma, z : \SigI{t}{x : A}{B} \vdash C : s \\
    \Gamma ; \Delta_1 \vdash m : \SigI{t}{x : A}{B} \\
    \Gamma, x : A, y : B; \Delta_2, x \ty{r} A \vdash n : C[\pairI{x}{y}{t}/z] }
  { \Gamma ; \Delta_1 \dotcup \Delta_2 \vdash \SigElim{[z]C}{m}{[x,y]n} : C[m/z] }

  \inferrule
  { \Gamma ; \Delta \vdash m : A \\
    \Gamma ; \Delta \vdash n : B \\
    \Delta \triangleright t }
  { \Gamma ; \Delta \vdash \apair{m}{n}{t} : \with{A}{B}{t} }

  \inferrule
  { \Gamma ; \Delta \vdash m : \with{A}{B}{t} }
  { \Gamma ; \Delta \vdash \projL{m} : A }

  \inferrule
  { \Gamma ; \Delta \vdash m : \with{A}{B}{t} }
  { \Gamma ; \Delta \vdash \projR{m} : B }

  \inferrule
  { \Gamma \vdash B : s \\
    \Gamma ; \Delta \vdash m : A \\
    A \simeq B }
  { \Gamma ; \Delta \vdash m : B }
\end{mathpar}

\newpage

\section{Erasure}

\subsection*{Erasure Relation}
\begin{mathpar}
  \inferrule
  { \Gamma, x : A ; \Delta, x \ty{s} A \vdash \\
    \Delta \triangleright \Un }
  { \Gamma, x : A ; \Delta, x \ty{s} A  \vdash x \sim x : A }

  \inferrule
  { \Gamma, x : A ; \Delta, x \ty{s} A \vdash m \sim m' : B \\
    \Delta \triangleright t }
  { \Gamma ; \Delta \vdash
    \lamR{t}{x : A}{m} \sim \lamR{t}{x : \square}{m'} : \PiR{t}{x : A}{B} }

  \inferrule
  { \Gamma, x : A ; \Delta \vdash m \sim m' : B \\
    \Delta \triangleright t }
  { \Gamma ; \Delta \vdash
    \lamI{t}{x : A}{m} \sim \lamI{t}{x : \square}{m'} : \PiI{t}{x : A}{B} }

  \inferrule
  { \Gamma ; \Delta_1 \vdash m \sim m' : \PiR{t}{x : A}{B} \\
    \Gamma ; \Delta_2 \vdash n \sim n' : A }
  { \Gamma ; \Delta_1 \dotcup \Delta_2 \vdash m\ n \sim m'\ n' : B[n/x] }

  \inferrule
  { \Gamma ; \Delta \vdash m \sim m' : \PiI{t}{x : A}{B} \\
    \Gamma \vdash n : A }
  { \Gamma ; \Delta \vdash m\ n \sim m'\ \square : B[n/x] }

  \inferrule
  { \Gamma \vdash \SigR{t}{x : A}{B} : t \\
    \Gamma ; \Delta_1 \vdash m \sim m' : A \\
    \Gamma ; \Delta_2 \vdash n \sim n' : B[m/x] }
  { \Gamma ; \Delta_1 \dotcup \Delta_2 \vdash
    \pairR{m}{n}{t} \sim \pairR{m'}{n'}{t} : \SigR{t}{x : A}{B} }

  \inferrule
  { \Gamma \vdash \SigI{t}{x : A}{B} : t \\
    \Gamma ; \Delta \vdash m \sim m' : A \\
    \Gamma \vdash n : B[m/x] }
  { \Gamma ; \Delta \vdash
    \pairI{m}{n}{t} \sim \pairI{m'}{\square}{t} : \SigI{t}{x : A}{B} }

  \inferrule
  { \Gamma, z : \SigR{t}{x : A}{B} \vdash C : s \\
    \Gamma ; \Delta_1 \vdash m \sim m' : \SigR{t}{x : A}{B} \\
    \Gamma, x : A, y : B ; \Delta_2, x \ty{r1} A, y \ty{r2} B \vdash n \sim n' : C[\pairR{x}{y}{t}/z] }
  { \Gamma ; \Delta_1 \dotcup \Delta_2 \vdash
    \SigElim{[z]C}{m}{[x,y]n} \sim \SigElim{[z]\square}{m'}{[x,y]n'} : C[m/z] }

  \inferrule
  { \Gamma, z : \SigI{t}{x : A}{B} \vdash C : s \\
    \Gamma ; \Delta_1 \vdash m \sim m' : \SigI{t}{x : A}{B} \\
    \Gamma, x : A, y : B ; \Delta_2, x \ty{r} A \vdash n \sim n' : C[\pairI{x}{y}{t}/z] }
  { \Gamma ; \Delta_1 \dotcup \Delta_2 \vdash
    \SigElim{[z]C}{m}{[x,y]n} \sim \SigElim{[z]\square}{m'}{[x,y]n'} : C[m/z] }

  \inferrule
  { \Gamma ; \Delta \vdash m \sim m' : A \\
    \Gamma ; \Delta \vdash n \sim n' : B \\
    \Delta \triangleright t }
  { \Gamma ; \Delta \vdash \apair{m}{n}{t} \sim \apair{m'}{n'}{t} : \with{A}{B}{t} }

  \inferrule
  { \Gamma ; \Delta \vdash m \sim m' : \with{A}{B}{t} }
  { \Gamma ; \Delta \vdash \projL{m} \sim \projL{m'} : A }

  \inferrule
  { \Gamma ; \Delta \vdash m \sim m' : \with{A}{B}{t} }
  { \Gamma ; \Delta \vdash \projR{m} \sim \projR{m'} : B }

  \inferrule
  { \Gamma \vdash B : s \\
    \Gamma ; \Delta \vdash m \sim m' : A \\
    A \simeq B }
  { \Gamma ; \Delta \vdash m \sim m' : B }
\end{mathpar}

\newpage

\section{Static Semantics}
\subsection*{Static Reduction}
\begin{mathpar}
  \inferrule
  { A \leadsto A' }
  { \PiR{t}{x : A}{B} \leadsto \PiR{t}{x : A'}{B} }

  \inferrule
  { B \leadsto B' }
  { \PiR{t}{x : A}{B} \leadsto \PiR{t}{x : A}{B'} }

  \inferrule
  { A \leadsto A' }
  { \PiI{t}{x : A}{B} \leadsto \PiI{t}{x : A'}{B} }

  \inferrule
  { B \leadsto B' }
  { \PiI{t}{x : A}{B} \leadsto \PiI{t}{x : A}{B'} }

  \inferrule
  { A \leadsto A' }
  { \lamR{t}{x : A}{m} \leadsto \lamR{t}{x : A'}{m} }

  \inferrule
  { m \leadsto m' }
  { \lamR{t}{x : A}{m} \leadsto \lamR{t}{x : A}{m'} }

  \inferrule
  { A \leadsto A' }
  { \lamI{t}{x : A}{m} \leadsto \lamI{t}{x : A'}{m} }

  \inferrule
  { m \leadsto m' }
  { \lamI{t}{x : A}{m} \leadsto \lamI{t}{x : A}{m'} }

  \inferrule
  { m \leadsto m' }
  { m\ n \leadsto m'\ n }

  \inferrule
  { n \leadsto n' }
  { m\ n \leadsto m\ n' }

  \inferrule
  { }
  { (\lamR{t}{x : A}{m})\ n \leadsto m[n/x] }

  \inferrule
  { }
  { (\lamI{t}{x : A}{m})\ n \leadsto m[n/x] }

  \inferrule
  { A \leadsto A' }
  { \SigR{t}{x : A}{B} \leadsto \SigR{t}{x : A'}{B} }

  \inferrule
  { B \leadsto B' }
  { \SigR{t}{x : A}{B} \leadsto \SigR{t}{x : A}{B'} }

  \inferrule
  { A \leadsto A' }
  { \SigI{t}{x : A}{B} \leadsto \SigI{t}{x : A'}{B} }

  \inferrule
  { B \leadsto B' }
  { \SigI{t}{x : A}{B} \leadsto \SigI{t}{x : A}{B'} }

  \inferrule
  { m \leadsto m' }
  { \pairR{m}{n}{t} \leadsto \pairR{m'}{n}{t} }

  \inferrule
  { n \leadsto n' }
  { \pairR{m}{n}{t} \leadsto \pairR{m}{n'}{t} }

  \inferrule
  { m \leadsto m' }
  { \pairI{m}{n}{t} \leadsto \pairI{m'}{n}{t} }

  \inferrule
  { n \leadsto n' }
  { \pairI{m}{n}{t} \leadsto \pairI{m}{n'}{t} }

  \inferrule
  { A \leadsto A' }
  { \SigElim{[z]A}{m}{[x,y]n} \leadsto \SigElim{[z]A'}{m}{[x,y]n} }

  \inferrule
  { m \leadsto m' }
  { \SigElim{[z]A}{m}{[x,y]n} \leadsto \SigElim{[z]A}{m'}{[x,y]n} }

  \inferrule
  { n \leadsto n' }
  { \SigElim{[z]A}{m}{[x,y]n} \leadsto \SigElim{[z]A}{m}{[x,y]n'} }

  \inferrule
  { }
  { \SigElim{[z]A}{\pairR{m_1}{m_2}{t}}{[x,y]n} \leadsto n[m_1/x,m_2/y] }

  \inferrule
  { }
  { \SigElim{[z]A}{\pairI{m_1}{m_2}{t}}{[x,y]n} \leadsto n[m_1/x,m_2/y] }

  \inferrule
  { A \leadsto A' }
  { \with{A}{B}{t} \leadsto \with{A'}{B}{t} }

  \inferrule
  { B \leadsto B' }
  { \with{A}{B}{t} \leadsto \with{A}{B'}{t} }

  \inferrule
  { m \leadsto m' }
  { \apair{m}{n}{t} \leadsto \apair{m'}{n}{t} }

  \inferrule
  { n \leadsto n' }
  { \apair{m}{n}{t} \leadsto \apair{m}{n'}{t} }

  \inferrule
  { m \leadsto m' }
  { \projL{m} \leadsto \projL{m'} }

  \inferrule
  { m \leadsto m' }
  { \projR{m} \leadsto \projR{m'} }

  \inferrule
  { }
  { \projL{\apair{m}{n}{t}} \leadsto m }

  \inferrule
  { }
  { \projR{\apair{m}{n}{t}} \leadsto n }

  \inferrule
  { A \leadsto A' }
  { \iden{A}{m}{n} \leadsto \iden{A'}{m}{n} }

  \inferrule
  { m \leadsto m' }
  { \iden{A}{m}{n} \leadsto \iden{A}{m'}{n} }

  \inferrule
  { n \leadsto n' }
  { \iden{A}{m}{n} \leadsto \iden{A}{m}{n'} }

  \inferrule
  { A \leadsto A' }
  { \idenElim{[x,y,p]A}{[z]H}{P} \leadsto \idenElim{[x,y,p]A'}{[z]H}{P} }

  \inferrule
  { H \leadsto H' }
  { \idenElim{[x,y,p]A}{[z]H}{P} \leadsto \idenElim{[x,y,p]A}{[z]H'}{P} }

  \inferrule
  { P \leadsto P' }
  { \idenElim{[x,y,p]A}{[z]H}{P} \leadsto \idenElim{[x,y,p]A}{[z]H}{P'} }

  \inferrule
  { }
  { \idenElim{[x,y,p]A}{[z]H}{\refl{m}} \leadsto H[m/z] }
\end{mathpar}

\subsection*{Conversion}
\begin{mathpar}
  \inferrule
  {  }
  { A \simeq A }

  \inferrule
  { A \simeq B \\ B \leadsto C }
  { A \simeq C }

  \inferrule
  { A \simeq B \\ C \leadsto B }
  { A \simeq C }
\end{mathpar}

\newpage

\section{Dynamic Semantics}

\subsection*{Value}
\begin{mathpar}
  \inferrule
  { }
  { x \val }

  \inferrule
  { }
  { \lamR{t}{x : A}{m} \val }

  \inferrule
  { }
  { \lamI{t}{x : A}{m} \val }

  \inferrule
  { u \val \\ v \val }
  { \pairR{u}{v}{t} \val }

  \inferrule
  { v \val }
  { \pairI{v}{m}{t} \val }

  \inferrule
  { }
  { \apair{m}{n}{t} \val }
\end{mathpar}

\subsection*{Dynamic Reduction}
\begin{mathpar}
  \inferrule
  { m \Leadsto m' }
  { m\ n \Leadsto m'\ n }

  \inferrule
  { n \Leadsto n' }
  { m\ n \Leadsto m\ n' }

  \inferrule
  { v \val }
  { (\lamR{t}{x : A}{m})\ v \Leadsto m[v/x] }

  \inferrule
  { }
  { (\lamI{t}{x : A}{m})\ n \Leadsto m[n/x] }

  \inferrule
  { m \Leadsto m' }
  { \pairR{m}{n}{t} \Leadsto \pairR{m'}{n}{t} }

  \inferrule
  { n \Leadsto n' }
  { \pairR{m}{n}{t} \Leadsto \pairR{m}{n'}{t} }

  \inferrule
  { m \Leadsto m' }
  { \pairI{m}{n}{t} \Leadsto \pairI{m'}{n}{t} }

  \inferrule
  { m \Leadsto m' }
  { \SigElim{[z]A}{m}{[x,y]n} \Leadsto \SigElim{[z]A}{m'}{[x,y]n} }

  \inferrule
  { u \val \\ v \val }
  { \SigElim{[z]A}{\pairR{u}{v}{t}}{[x,y]n} \Leadsto n[u/x,v/y] }

  \inferrule
  { v \val }
  { \SigElim{[z]A}{\pairI{v}{m}{t}}{[x,y]n} \Leadsto n[v/x,m/y] }

  \inferrule
  { m \Leadsto m' }
  { \projL{m} \Leadsto \projL{m'} }

  \inferrule
  { m \Leadsto m' }
  { \projR{m} \Leadsto \projR{m'} }

  \inferrule
  { }
  { \projL{\apair{m}{n}{t}} \Leadsto m }

  \inferrule
  { }
  { \projR{\apair{m}{n}{t}} \Leadsto n }
\end{mathpar}

\newpage

\section{Meta Theory}

\subsection*{Static Meta Theory}
\begin{theorem}[Confluence]
  If $m \leadsto^{*} m_{1}$ and $m \leadsto^{*} m_{2}$, then there exists $n$ such that $m_{1} \leadsto^{*} n$ and $m_{2} \leadsto^{*} n$.
\end{theorem}

\begin{theorem}[Conversion]
  Conversion $\simeq$ is an equivalence relation.
\end{theorem}

\begin{theorem}[Static Validity]
  For any static typing $\Gamma \vdash m : A$, there exists sort $s$ such that $\Gamma \vdash A : s$ is derivable.
\end{theorem}

\begin{theorem}[Sort Uniqueness]
  If there are static typings $\Gamma \vdash A : s$ and $\Gamma \vdash A : t$, then $s = t$.
\end{theorem}

\begin{theorem}[Static Subject Reduction]
  If there is static typing $\Gamma \vdash m : A$ and static reduction $m \leadsto n$, then $\Gamma \vdash n : A$ is derivable.
\end{theorem}

\begin{theorem}[Static Normalization]
  For any $m$ with static typing $\Gamma \vdash m : A$, it is strongly normalizing.
\end{theorem}

\subsection*{Dynamic Meta Theory}
\begin{theorem}[Dynamic Reflection]
  For any dynamic typing $\Gamma ; \Delta \vdash m : A$, static typing $\Gamma \vdash m : A$ is derivable.
\end{theorem}

\begin{theorem}[Value Stability]
  If there is value $v$ with dynamic typing $\Gamma ; \Delta \vdash v : A$ and $\Gamma \vdash A : s$, then $\Delta \triangleright s$.
\end{theorem}

\begin{theorem}[Dynamic Subject Reduction]
  If there is dynamic typing $\Gamma ; \Delta \vdash m : A$ and dynamic reduction $m \Leadsto n$, then $\Gamma ; \Delta \vdash n : A$ is derivable.
\end{theorem}

\begin{theorem}[Dynamic Progress]
  If there is dynamic typing $\epsilon ; \epsilon \vdash m : A$, then $m$ is a value or there exists $n$ such that $m \Leadsto n$.
\end{theorem}

\subsection*{Erasure-Dynamic Meta Theory}
\begin{theorem}[Erasure Existence]
  For any dynamic typing $\Gamma ; \Delta \vdash m : A$, there exists $m'$ such that erasure relation $\Gamma ; \Delta \vdash m \sim m' : A$ is derivable.
\end{theorem}

\begin{theorem}[Erasure Subject Reduction]
  For any erasure relation $\Gamma ; \Delta \vdash m \sim m' : A$ and dynamic reduction $m' \Leadsto n'$, there exists $n$ such that the following diagram commutes.
  \begin{center}
    \begin{tikzcd}
      {\Gamma ; \Delta } &[-18pt] m &[-7pt] {m'} &[-20pt] A \\
      {\Gamma ; \Delta} &[-18pt] n &[-7pt] {n'} &[-20pt] A
      \arrow["\sim"{description}, draw=none, from=1-2, to=1-3]
      \arrow["\vdash"{description}, draw=none, from=1-1, to=1-2]
      \arrow["{:}"{description}, draw=none, from=1-3, to=1-4]
      \arrow["\Leadsto"{marking}, draw=none, from=1-2, to=2-2]
      \arrow["\Leadsto"{marking}, draw=none, from=1-3, to=2-3]
      \arrow["\vdash"{description}, draw=none, from=2-1, to=2-2]
      \arrow["{:}"{description}, draw=none, from=2-3, to=2-4]
      \arrow["\sim"{marking}, draw=none, from=2-2, to=2-3]
      \arrow[draw=none, from=2-3, to=2-4]
    \end{tikzcd}
  \end{center}
\end{theorem}

\begin{theorem}[Erasure Progress]
  For any erasure relation $\epsilon ; \epsilon \vdash m \sim m' : A$, then $m'$ is a value or there exists $n'$ such that $m' \Leadsto n'$.
\end{theorem}

\end{document}
